theories/zoo_std/mutex__code.v
@@ -14,7 +14,7 @@ Definition mutex_create : val :=
 
 Definition mutex_lock : val :=
   rec: "lock" "t" =>
-    ifnot: CAS "t".[contents] #false #true then (
+    if: ~ CAS "t".[contents] #false #true then (
       Yield ;;
       "lock" "t"
     ).
